feat: add getKey?

src/Std/Data/DHashMap/Basic.lean
@@ -98,6 +98,9 @@ instance [BEq α] [Hashable α] : Inhabited (DHashMap α β) where
     (a : α) : Option (β a) :=
   Raw₀.get? ⟨m.1, m.2.size_buckets_pos⟩ a
 
+@[inline, inherit_doc Raw.getKey?] def getKey? (m : DHashMap α β) (a : α) : Option α :=
+  Raw₀.getKey? ⟨m.1, m.2.size_buckets_pos⟩ a
+
 @[inline, inherit_doc Raw.contains] def contains (m : DHashMap α β) (a : α) :
     Bool :=
   Raw₀.contains ⟨m.1, m.2.size_buckets_pos⟩ a
