src/Std/Data/DHashMap/Internal/List/Associative.lean
@@ -527,6 +527,33 @@ theorem getValue!_eq_getValueD_default [BEq α] [Inhabited β] {l : List ((_ : �
 end
 
 /-- Internal implementation detail of the hash map -/
+def getKey? [BEq α] (a : α) : List ((a : α) × β a) → Option α
+  | [] => none
+  | ⟨k, _⟩ :: l => bif k == a then some k else getKey? a l
+
+@[simp] theorem getKey?_nil [BEq α] {a : α} :
+    getKey? a ([] : List ((a : α) × β a)) = none := rfl
+@[simp] theorem getKey?_cons [BEq α] {l : List ((a : α) × β a)} {k a : α} {v : β k} :
+    getKey? a (⟨k, v⟩ :: l) = bif k == a then some k else getKey? a l := rfl
+
+theorem getKey?_cons_of_true [BEq α] {l : List ((a : α) × β a)} {k a : α} {v : β k} (h : k == a) :
+    getKey? a (⟨k, v⟩ :: l) = some k := by
+  simp [h]
+
+theorem getKey?_cons_of_false [BEq α] {l : List ((a : α) × β a)} {k a : α} {v : β k}
+    (h : (k == a) = false) : getKey? a (⟨k, v⟩ :: l) = getKey? a l := by
+  simp [h]
+
+theorem getKey?_eq_getEntry? [BEq α] {l : List ((a : α) × β a)} {a : α} :
+    getKey? a l = (getEntry? a l).map (·.1) := by
+  induction l using assoc_induction
+  · simp
+  · next k v l ih =>
+    cases h : k == a
+    · rw [getEntry?_cons_of_false h, getKey?_cons_of_false h, ih]
+    · rw [getEntry?_cons_of_true h, getKey?_cons_of_true h, Option.map_some']
+
+/-- Internal implementation detail of the hash map -/
 def replaceEntry [BEq α] (k : α) (v : β k) : List ((a : α) × β a) → List ((a : α) × β a)
   | [] => []
   | ⟨k', v'⟩ :: l => bif k' == k then ⟨k, v⟩ :: l else ⟨k', v'⟩ :: replaceEntry k v l
@@ -642,6 +669,18 @@ theorem getValueCast?_replaceEntry [BEq α] [LawfulBEq α] {l : List ((a : α) �
         getValueCast?_eq_getEntry?]
     · rw [Option.dmap_congr (getEntry?_replaceEntry_of_false (Bool.eq_false_iff.2 h)),
         getValueCast?_eq_getEntry?]
+
+theorem getKey?_replaceEntry [BEq α] [PartialEquivBEq α] {l : List ((a : α) × β a)} {a k : α}
+    {v : β k} : getKey? a (replaceEntry k v l) =
+      if containsKey k l ∧ k == a then some k else getKey? a l := by
+  rw [getKey?_eq_getEntry?]
+  split
+  · next h => simp [getEntry?_replaceEntry_of_true h.1 h.2]
+  · next h =>
+    simp only [Decidable.not_and_iff_or_not_not] at h
+    rcases h with h|h
+    · rw [getEntry?_replaceEntry_of_containsKey_eq_false (Bool.eq_false_iff.2 h), getKey?_eq_getEntry?]
+    · rw [getEntry?_replaceEntry_of_false (Bool.eq_false_iff.2 h), getKey?_eq_getEntry?]
 
 @[simp]
 theorem containsKey_replaceEntry [BEq α] [PartialEquivBEq α] {l : List ((a : α) × β a)} {a k : α}
@@ -974,6 +1013,25 @@ theorem getValueD_insertEntry_self {β : Type v} [BEq α] [EquivBEq α] {l : Lis
     {k : α} {fallback v : β} : getValueD k (insertEntry k v l) fallback = v := by
   simp [getValueD_insertEntry, BEq.refl]
 
+theorem getKey?_insertEntry [BEq α] [PartialEquivBEq α] {l : List ((a : α) × β a)} {k a : α}
+    {v : β k} : getKey? a (insertEntry k v l) = if k == a then some k else getKey? a l := by
+  cases hl : containsKey k l
+  · simp [insertEntry_of_containsKey_eq_false hl]
+  · rw [insertEntry_of_containsKey hl, getKey?_replaceEntry, hl]
+    split <;> simp_all
+
+theorem getKey?_insertEntry_self [BEq α] [EquivBEq α] {l : List ((a : α) × β a)} {k : α}
+    {v : β k} : getKey? k (insertEntry k v l) = some k := by
+  simp [getKey?_insertEntry]
+
+theorem containsKey_eq_isSome_getKey? [BEq α] [PartialEquivBEq α] {l : List ((a : α) × β a)}
+    {a : α} : containsKey a l = (getKey? a l).isSome := by
+  simp [containsKey_eq_isSome_getEntry?, getKey?_eq_getEntry?]
+
+theorem getKey?_eq_none [BEq α] [PartialEquivBEq α] {l : List ((a : α) × β a)} {a : α}
+    (h : containsKey a l = false) : getKey? a l = none := by
+  rwa [← Option.not_isSome_iff_eq_none, ← containsKey_eq_isSome_getKey?, Bool.not_eq_true]
+
 @[local simp]
 theorem containsKey_insertEntry [BEq α] [PartialEquivBEq α] {l : List ((a : α) × β a)} {k a : α}
     {v : β k} : containsKey a (insertEntry k v l) = ((k == a) || containsKey a l) := by
@@ -1058,6 +1116,14 @@ theorem getValue?_insertEntryIfNew {β : Type v} [BEq α] [PartialEquivBEq α] {
       if k == a ∧ containsKey k l = false then some v else getValue? a l := by
   simp [getValue?_eq_getEntry?, getEntry?_insertEntryIfNew,
       apply_ite (Option.map (fun (y : ((_ : α) × β)) => y.2))]
+
+theorem getKey?_insertEntryIfNew [BEq α] [PartialEquivBEq α] {l : List ((a : α) × β a)} {k a : α}
+    {v : β k} : getKey? a (insertEntryIfNew k v l) =
+      if k == a ∧ containsKey k l = false then some k else getKey? a l := by
+  cases h : containsKey k l
+  · rw [insertEntryIfNew_of_containsKey_eq_false h]
+    split <;> simp_all
+  · simp [insertEntryIfNew_of_containsKey h]
 
 theorem containsKey_insertEntryIfNew [BEq α] [PartialEquivBEq α] {l : List ((a : α) × β a)}
     {k a : α} {v : β k} :
@@ -1253,6 +1319,18 @@ theorem getValue?_eraseKey [BEq α] [PartialEquivBEq α] {l : List ((_ : α) × 
 
 end
 
+theorem getKey?_eraseKey [BEq α] [PartialEquivBEq α] {l : List ((a : α) × β a)} {k a : α}
+    (hl : DistinctKeys l) :
+    getKey? a (eraseKey k l) = if k == a then none else getKey? a l := by
+  rw [getKey?_eq_getEntry?, getEntry?_eraseKey hl]
+  by_cases h : k == a
+  . simp [h]
+  . simp [h, getKey?_eq_getEntry?]
+
+theorem getKey?_eraseKey_self [BEq α] [PartialEquivBEq α] {l : List ((a : α) × β a)} {k : α}
+    (hl : DistinctKeys l) : getKey? k (eraseKey k l) = none := by
+  simp [getKey?_eq_getEntry?, getEntry?_eraseKey_self hl]
+
 theorem containsKey_eraseKey_self [BEq α] [PartialEquivBEq α] {l : List ((a : α) × β a)} {k : α}
     (h : DistinctKeys l) : containsKey k (eraseKey k l) = false := by
   simp [containsKey_eq_isSome_getEntry?, getEntry?_eraseKey_self h]
@@ -1412,6 +1490,10 @@ theorem getValueD_of_perm [BEq α] [PartialEquivBEq α] {l l' : List ((_ : α) �
 
 end
 
+theorem getKey?_of_perm [BEq α] [PartialEquivBEq α] {l l' : List ((a : α) × β a)} {a : α}
+    (hl : DistinctKeys l) (h : Perm l l') : getKey? a l = getKey? a l' := by
+  rw [getKey?_eq_getEntry?, getKey?_eq_getEntry?, getEntry?_of_perm hl h]
+
 theorem perm_cons_getEntry [BEq α] {l : List ((a : α) × β a)} {a : α} (h : containsKey a l) :
     ∃ l', Perm l (getEntry a l h :: l') := by
   induction l using assoc_induction
@@ -1520,6 +1602,11 @@ theorem getValueCast_append_of_containsKey_eq_false [BEq α] [LawfulBEq α]
       getValueCast a l ((containsKey_append_of_not_contains_right hl').symm.trans h) := by
   rw [← Option.some_inj, ← getValueCast?_eq_some_getValueCast, ← getValueCast?_eq_some_getValueCast,
     getValueCast?_append_of_containsKey_eq_false hl']
+
+theorem getKey?_append_of_containsKey_eq_false [BEq α] [PartialEquivBEq α]
+    {l l' : List ((a : α) × β a)} {a : α} (hl' : containsKey a l' = false) :
+    getKey? a (l ++ l') = getKey? a l := by
+  simp [getKey?_eq_getEntry?, getEntry?_eq_none.2 hl']
 
 theorem replaceEntry_append_of_containsKey_left [BEq α] {l l' : List ((a : α) × β a)} {k : α}
     {v : β k} (h : containsKey k l) : replaceEntry k v (l ++ l') = replaceEntry k v l ++ l' := by
